coq_inference/classical.v
@@ -605,7 +605,7 @@ Module ClassicalProperties(L : LanguageDef).
   Hint Resolve or_associative : chainmail_db.
 
   Lemma and_distributive_1:
-    forall M A1 A2 A3, entails M ((A1 ∨ A2) ∧ A3) ((A1 ∧ A3) ∨ (A2 ∧ A3)).
+    forall M A1 A2 A3, M ⊢ ((A1 ∨ A2) ∧ A3) ⊇ ((A1 ∧ A3) ∨ (A2 ∧ A3)).
   Proof.
     intros;
       apply ent;
@@ -620,7 +620,7 @@ Module ClassicalProperties(L : LanguageDef).
   Hint Resolve and_distributive_1 : chainmail_db.
 
   Lemma and_distributive_2:
-    forall M A1 A2 A3, entails M ((A1 ∧ A3) ∨ (A2 ∧ A3)) ((A1 ∨ A2) ∧ A3).
+    forall M A1 A2 A3, M ⊢ ((A1 ∧ A3) ∨ (A2 ∧ A3)) ⊇ ((A1 ∨ A2) ∧ A3).
   Proof.
     intros;
       apply ent;
@@ -972,6 +972,58 @@ Module ClassicalProperties(L : LanguageDef).
            | [H : ?M1 ◎ ?σ ⊨ (a_exp (e_false)) |- ?P] =>
              apply (false_not_satisfied_corollary M1 σ P H)
            end.
+
+
+
+  Lemma and_distributive_trans_1:
+    forall M A1 A2 A3 A, M ⊢ ((A1 ∨ A2) ∧ A3) ⊇ A ->
+                    M ⊢ ((A1 ∧ A3) ∨ (A2 ∧ A3)) ⊇ A.
+  Proof.
+    intros.
+    apply ent;
+      intros.
+    repeat a_prop.
+    disj_split.
+    a_prop.
+    inversion H;
+      subst.
+    eapply H3;
+      eauto;
+    auto with chainmail_db.
+    a_prop.
+    inversion H;
+      subst.
+    eapply H3;
+      eauto.
+    auto with chainmail_db.
+  Qed.
+
+  Hint Resolve and_distributive_trans_1 : chainmail_db.
+
+  Lemma and_distributive_trans_2:
+    forall M A1 A2 A3 A, M ⊢ ((A1 ∧ A3) ∨ (A2 ∧ A3)) ⊇ A ->
+                    M ⊢ ((A1 ∨ A2) ∧ A3) ⊇ A.
+  Proof.
+    intros.
+    apply ent;
+      intros.
+    repeat a_prop.
+    disj_split.
+    a_prop.
+    inversion H;
+      subst.
+    eapply H3;
+      eauto;
+    auto with chainmail_db.
+    a_prop.
+    inversion H;
+      subst.
+    eapply H3;
+      eauto.
+    auto with chainmail_db.
+  Qed.
+
+  Hint Resolve and_distributive_trans_2 : chainmail_db.
 
   Close Scope chainmail_scope.
   Close Scope reduce_scope.
